Example.lean
@@ -1,12 +1,14 @@
 variable {p q r : Prop}
 
 theorem imp_trans (hpq : p → q) (hqr : q → r) : p → r := by
-  intro hp
-  exact hqr (hpq hp)
+  intro h
+  apply hqr
+  apply hpq
+  apply h
 
 theorem or_comm' (h : p ∨ q) : q ∨ p := by
-  rcases h with h | h
+  rcases h
   right
-  exact h
+  assumption
   left
-  exact h
+  assumption
