LSPLogAnalyzer/Utils.lean
@@ -1,0 +1,79 @@
+import Lean
+import LSPLogAnalyzer.Definitions
+
+open Lean.Json
+open Lean.FromJson
+open Lean.JsonRpc
+open Lean.Lsp
+
+namespace LSPLogAnalyzer
+
+open IO.FS in
+def fileStream (filename : System.FilePath) : IO Stream := do
+  return .ofHandle (← Handle.mk filename Mode.read)
+
+def parseLogLine (line : String) : Except String LogEntry := do
+  Lean.fromJson? (← parse line)
+
+def ensureFile (uri : String) : TrackerM FileState := do
+  let st ← get
+  match st.files.get? uri with
+  | some fs => return fs
+  | none =>
+    let fs : FileState := {}
+    set { st with files := st.files.insert uri fs }
+    return fs
+
+def messageSummary : Message → String
+  | .request id method@"$/lean/rpc/call" (some params) =>
+      let rpcmethod := params.toJson.getObjValAs? String "method" |>.toOption
+      s!"request {id} - {method} {rpcmethod.getD "unknown method"}"
+  | .request id method _params? => s!"request {id} - {method}"
+  | .notification method _params? => s!"notification - {method}"
+  | .response id _result => s!"response {id}"
+  | .responseError id _errCode _msg _params? => s!"response error {id}"
+
+def logEntrySummary (e : LogEntry) : String := messageSummary e.msg
+
+def getLine : TrackerM Nat := do
+  return (← get).line
+
+def collectLogEntries (path : System.FilePath) : IO (Array LogEntry) := do
+  let log ← IO.FS.readFile path
+  let log := log.trimRight
+  let entries := log.splitOn "\n" |>.toArray
+  let entries := entries.map parse
+  let entries ← IO.ofExcept <| entries.mapM id
+  IO.ofExcept <| entries.mapM fromJson?
+
+def modifyFileState (uri : Uri) (fs : FileState) : TrackerM Unit := do
+  modify fun s => { s with files := s.files.insert uri fs }
+
+def locatePos (defs : Array Definition) (pos : Lean.Lsp.Position)
+    (lo : Nat := 0) (hi : Nat := defs.size) : Option (Nat × Definition) :=
+  if hi ≤ lo then none
+  else
+    let m := (lo + hi) / 2
+    defs[m]? >>= fun d =>
+      if pos ∈ d.range then
+        (m, d)
+      else if pos < d.range.start then
+        locatePos defs pos lo m
+      else
+        locatePos defs pos (m+1) hi
+  termination_by hi - lo
+
+def relativePos (origin pos : Position) : Position :=
+  if origin.line == pos.line then
+    ⟨0, pos.character - origin.character⟩
+  else
+    ⟨pos.line - origin.line, pos.character⟩
+
+def relativeRange (enclosing inner : Range) : Range :=
+  ⟨relativePos enclosing.start inner.start, relativePos enclosing.start inner.end⟩
+
+def updateDefDiag (defn : Definition) (diag : Diagnostic) : Definition :=
+  let diag := { diag with range := relativeRange defn.range diag.range }
+  { defn with diags := defn.diags.push diag }
+
+end LSPLogAnalyzer
